src/parser/parse.mly
@@ -96,7 +96,7 @@ let none_to_empty_list x =
 %token PRIVATE REIFIABLE REFLECTABLE REIFY RANGE_OF SET_RANGE_OF LBRACE_COLON_PATTERN PIPE_RIGHT
 %token NEW_EFFECT SUB_EFFECT LAYERED_EFFECT POLYMONADIC_BIND POLYMONADIC_SUBCOMP SPLICE SPLICET SQUIGGLY_RARROW TOTAL
 %token REQUIRES ENSURES DECREASES LBRACE_COLON_WELL_FOUNDED
-%token MINUS COLON_EQUALS QUOTE BACKTICK_AT BACKTICK_HASH
+%token MINUS COLON_EQUALS BACKTICK_AT BACKTICK_HASH
 %token BACKTICK UNIV_HASH
 %token BACKTICK_PERC
 
@@ -120,7 +120,7 @@ let none_to_empty_list x =
 %left     OPINFIX0d
 %left     PIPE_RIGHT
 %right    OPINFIX1
-%left     OPINFIX2 MINUS QUOTE
+%left     OPINFIX2 MINUS
 %left     OPINFIX3
 %left     BACKTICK
 %right    OPINFIX4
@@ -1073,13 +1073,8 @@ tmEqWith(X):
       { mk_term (Op(mk_ident("-", rhs parseState 2), [e1; e2])) (rhs2 parseState 1 3) Un}
   | MINUS e=tmEqWith(X)
       { mk_uminus e (rhs parseState 1) (rhs2 parseState 1 2) Expr }
-  | QUOTE e=tmEqWith(X)
-      { mk_term (Quote (e, Dynamic)) (rhs2 parseState 1 3) Un }
   | BACKTICK e=tmEqWith(X)
-      { mk_term (Quote (e, Static)) (rhs2 parseState 1 3) Un }
-  | BACKTICK_AT e=atomicTerm
-      { let q = mk_term (Quote (e, Dynamic)) (rhs2 parseState 1 3) Un in
-        mk_term (Antiquote q) (rhs2 parseState 1 3) Un }
+      { mk_term (Quote e) (rhs2 parseState 1 3) Un }
   | BACKTICK_HASH e=atomicTerm
       { mk_term (Antiquote e) (rhs2 parseState 1 3) Un }
   | e=tmNoEqWith(X)
