src/typechecker/FStar.TypeChecker.Normalize.fst
@@ -361,10 +361,6 @@ let rec inline_closure_env cfg (env:env) stack t =
 
       | Tm_quoted (t', qi) ->
         let t =
-            match qi.qkind with
-            | Quote_dynamic ->
-              mk (Tm_quoted(non_tail_inline_closure_env cfg env t', qi)) t.pos
-            | Quote_static  ->
               let qi = S.on_antiquoted (non_tail_inline_closure_env cfg env) qi in
               mk (Tm_quoted(t', qi)) t.pos
         in
